

Ans. to the Q.no-A

Given,

$$z_1 = -1 + i$$

$$\frac{z_1}{3+4i} = m + in$$

$$\text{or, } \frac{-1+i}{3+4i} = m + in$$

$$\text{or, } m + in = \frac{(-1+i)(3-4i)}{(3+4i)(3-4i)}$$

$$\text{or, } m + in = \frac{(-1+i)(3-4i)}{9-16i^2}$$

[Multiplying
the numerator
and denominator
by $(3-4i)$]

$$\text{or, } m + in = \frac{-3 + 4i + 3i - 4i^2}{9+16}$$

$$\text{or, } m + in = \frac{1+7i}{25}$$

$$\text{or, } m + in = \frac{1}{25} + \frac{7}{25}i$$

$$\text{so, } m = \frac{1}{25}, n = \frac{7}{25}$$

Now,

$$m^4 - m^2n^2 + n^4 = \left(\frac{1}{25}\right)^4 - \left(\frac{1}{25}\right)^2 \times \left(\frac{7}{25}\right)^2 + \left(\frac{7}{25}\right)^4$$

$$= \frac{1}{25^4} - \frac{7^2}{25^4} + \frac{7^4}{25^4}$$

$$= \frac{1-7^2+7^4}{25^4} = \frac{2353}{390625} \quad (\text{Ans})$$

Ans. to the Q.no-B

Given,

$$z_1 = -1 + i$$

$$\bar{z}_1 = -1 - i \quad [\text{conjugate of } z_1]$$

$$\begin{aligned} \text{Now, modulus, } r &= \sqrt{(-1)^2 + (-1)^2} \\ &= \sqrt{2} \end{aligned}$$

$$\begin{aligned} \text{Argument, } \theta &= -\pi + \tan^{-1}\left(\frac{-1}{-1}\right) \quad [\text{since it lies in the 3rd quadrant.}] \\ &= -\pi + \tan^{-1}(1) \\ &= -\pi + \frac{\pi}{4} \\ &= -\frac{3\pi}{4} \end{aligned}$$

Now, expressing in polar form:

$$\begin{aligned} \bar{z}_1 &= r \cos \theta + i r \sin \theta \\ &= r (\cos \theta + i \sin \theta) \\ &= \sqrt{2} \left(\cos\left(-\frac{3\pi}{4}\right) + i \sin\left(-\frac{3\pi}{4}\right) \right) \\ &= \sqrt{2} \left(\cos \frac{3\pi}{4} + i \sin \frac{3\pi}{4} \right) \end{aligned}$$

$$\left[\begin{aligned} \because \sin(-\theta) &= -\sin \theta \\ \cos(-\theta) &= \cos \theta \end{aligned} \right]$$

Ans: to the Q.no-2

Given,

$$z_1 = -1 + i$$

Let,

$$x^2 = -1 + i = z_1$$

$$x = \sqrt{z_1}$$

Now,

$$x^2 = -1 + i$$

$$\text{or, } x^2 = \frac{1}{2}(-2 + 2i)$$

$$\text{or, } x = \frac{1}{2}(-2 + 2i \sqrt{\sqrt{2}+1} \times \sqrt{\sqrt{2}-1})$$

$$\text{or, } x = \frac{1}{2}(\cancel{\sqrt{2}-1} \sqrt{2}-1 - \sqrt{2}-1 + 2i \sqrt{(\sqrt{2}+1)(\sqrt{2}-1)})$$

$$\text{or, } x = \frac{1}{2} \left\{ (\sqrt{\sqrt{2}-1})^2 + i^2 (\sqrt{\sqrt{2}+1})^2 + 2 \cdot \sqrt{\sqrt{2}-1} \cdot i \sqrt{\sqrt{2}+1} \right\}$$

$$\text{or, } x^2 = \frac{1}{2} \left\{ (\sqrt{\sqrt{2}-1}) + (i \sqrt{\sqrt{2}+1}) \right\}^2$$

$$\text{or, } x = \pm \frac{1}{\sqrt{2}} (\sqrt{\sqrt{2}-1} + i \sqrt{\sqrt{2}+1})$$

$$\text{So, } \sqrt{z_1} = \pm \frac{1}{\sqrt{2}} \left\{ (\sqrt{2}-1)^{\frac{1}{2}} + i (\sqrt{2}+1)^{\frac{1}{2}} \right\}$$

Ans. to the Q no-D

Given,

$$z = x + iy$$

$$\text{and } z = p + p^{-1}$$

$$p = 3(\cos\theta + i\sin\theta)$$

$$\therefore z = 3(\cos\theta + i\sin\theta) + \frac{1}{3(\cos\theta + i\sin\theta)}$$

$$\text{or, } z = 3(\cos\theta + i\sin\theta) + \frac{(\cos\theta - i\sin\theta)}{3(\cos^2\theta - i^2\sin^2\theta)}$$

$$\text{or, } z = 3(\cos\theta + i\sin\theta) + \frac{(\cos\theta - i\sin\theta)}{3(\cos^2\theta + \sin^2\theta)}$$

$$\text{or, } z = 3(\cos\theta + i\sin\theta) + \frac{1}{3}(\cos\theta - i\sin\theta)$$

$$\text{or, } z = 3\cos\theta + \frac{1}{3}\cos\theta + 3i\sin\theta - \frac{1}{3}i\sin\theta$$

$$\text{or, } z = \frac{10}{3}\cos\theta + \frac{8}{3}i\sin\theta$$

$$\text{Thus, } \frac{10}{3}\cos\theta + \frac{8}{3}i\sin\theta = x + iy$$

$$\therefore x = \frac{10}{3}\cos\theta$$

$$y = \frac{8}{3}\sin\theta$$

Now,

$$\text{L.H.S} = \frac{9x^2}{100} + \frac{9y^2}{64} = \frac{9 \times \frac{10^2}{3^2} \cos^2\theta}{100} + \frac{9 \times \frac{8^2}{3^2} \sin^2\theta}{64}$$

$$= \cos^2\theta + \sin^2\theta$$

$$= 1 = \text{R.H.S} \quad \therefore \text{L.H.S} = \text{R.H.S}$$

$$\therefore \frac{9x^2}{100} + \frac{9y^2}{64} = 1 \quad [\text{proved}]$$

Ans. to the Q.no-E

Given,

$$z_1 = -1 + i$$

$$\therefore \bar{z}_1 = -1 - i$$

$$\therefore \frac{1}{2}(z_1 + \bar{z}_1) = \frac{1}{2}(-1 + i - 1 - i) = \frac{1}{2}(-2) = -1$$

$$\text{Now, } \frac{1}{2}(z_1 + \bar{z}_1) = a$$

$$\text{or, } a = -1$$

$$\text{or, } \sqrt[6]{a} = \sqrt[6]{-1}$$

$$\text{let, } x = \sqrt[6]{-1} = \sqrt[6]{a}$$

$$\therefore x^6 = -1$$

$$\text{or, } x^6 + 1 = 0$$

$$\text{or, } x^6 - i^2 = 0$$

$$\text{or, } (x^3)^2 - (i)^2 = 0$$

$$\text{or, } (x^3 - i)(x^3 + i) = 0$$

$$\text{Either } x^3 - i = 0 \quad \text{or} \quad x^3 + i = 0$$

$$\text{If } x^3 - i = 0$$

$$x^3 + i^3 = 0$$

$$\text{or, } (x+i)(x^2+i^2-xi) = 0$$

$$\text{or, } x+i = 0 \quad \text{or} \quad x^2+i^2-xi = 0$$

$$x = -i$$

$$x = \frac{i \pm \sqrt{i^2 - 4 \times 1 \times i^2}}{2}$$

$$= \frac{i \pm \sqrt{-1+4}}{2}$$

$$= \frac{i \pm \sqrt{3}}{2}$$

$$\text{If } x^3 + i = 0$$

$$x^3 - i^3 = 0$$

$$(x - i)(x^2 + i^2 + xi) = 0$$

$$x - i = 0$$

$$x = i$$

or

$$x^2 + i^2 + xi = 0$$

$$x = \frac{-i \pm \sqrt{i^2 - 4 \times 1 \times i^2}}{2}$$

$$= \frac{-i \pm \sqrt{-1 + 4}}{2}$$

$$= \frac{-i \pm \sqrt{3}}{2}$$

So, the required value of $\sqrt[6]{a}$

$$\sqrt[6]{a} = i, \frac{i \pm \sqrt{3}}{2}, \frac{-i \pm \sqrt{3}}{2} \quad (\text{Ans})$$